# 3.4N

1.  Each functioin can be written in the form $f(x) = a(x-p)(x-q)$, where $p > q$. Find the values of $a, p,$ and $q$ and then write down the coordinates of the $x$ and $y$ intercepts of the graph of $y=f(x)$.
- a. $f(x) = x^2 + 7x - 18$

    $(x-2)(x+9)$

- b. $f(x) = 3x^2 - 11x + 10$

    $-6, -5$<br>
    $3x^2 -6x -5x + 10$<br>
    $3x(x-2) + -5(x-2)$<br>
    $(3x-5)(x-2) = 3(x-2)(x-\frac{5}{3})$
    
 - d. $f(x) = -4x^2 +18x - 8$
 
    $-4x^2 + 2x + 16x - 8$<br>
    $-2x(2x - 1) + 8(2x - 1)$<br>
    $(2x-1)(-2x+8) = -4(x-4)(x-0.5)$
    
2. Each function can be written in the form $f(x) = ax^2 + bx + c$. Find the values of $a, b,$ and $c$ and then write down the coordinates of the $x$ and $y$ intercepts of the graph of $y=f(x)$.
- a. $f(x) = 4(x-1)(x+5)$

    $4(x^2 + 4x - 5) = 4x^2 + 16x - 20$

- b. $f(x) = -2(x+7)(x+1)$

    $-2(x^2 + 8x + 7) = -2x^2 - 16x -14$
    
 3. Each function can be written in the form $f(x) = ax^2 + bx + c$. Find the values of $a$, $b$, and $c$. Find the coordinates of the vertex and of the $y$ -intercept of the graph of $y=f(x)$.
 - a. $f(x) = -3(x+1)^2 - 6$
 
    Vertex: $(-1, -6)$<br>
    $y$ - intercept: $(0,-9)$
 
 - b. $f(x) = \frac{1}{2}(x-4)^2 + 3$
 
    Vertex: $(4,3)$<br>
    $y$ - intercept: $(0, 11)$

4. The functioni $f(x) = x^2 - 2x - 8$ can be written in the form $f(x) = a(x-p)(x-q)$, where $p > q$. 
- a. Find the values of 
- i. $a = 1$
- ii. $p = 4$
- iii. $a=-2$
- b. Write down the coordinates of the:
- i. x-intercepts: $(-2,4)$
- ii. y-intercepts: $(0,0)$

5. Let $f(x) = (x-3)^2 - 2$. Part of the graph of $y = f(x)$ is shown.
- a. The vertex of the graph of $y = f(x)$ is A.
- i. Write down the coordinates of A: $(3,-2)$
- ii. Write down the equation of the axis of symmetry for the graph of $y=f(x)$: $x = 3$
- b. Find the equation for the function $f$ in the form $f(x) = ax^2 + bx + c$.
- $x^2 -6x + 7$
- c. The coordinates of B are $(0,q)$. Write down the value of $q$: $7$
- e. The coordinates of C are $(p,q)$. Write down the value of $q$: $6$

6. Let $f(x) = x^2 - 2x - 3$ and $g(x) = x - 2$
- a. Let $h(x) = $(f \circ g)(x). Show that $h(x) = x^2 - 6x + 5$ <br>
         $h(x) = (x-2)^2 - 2(x-2) - 3 <br> =$ 
