# 3.5P

2. Solve by factorization:
- b. $3x^2 + 5x - 12 = 0$
    $e + s = 5, e \cdot s = -36$ <br> $e = 9, s = -4$ <br> $3x^2 + 9x - 4x - 12 = 0$ <br> $3x(x+3) - 4(x+3) = 0$ <br> $(3x-4)(x+3) = 0)$ <br> $x = -3, \frac{4}{3}$
- c. $4x^2 + 11x + 6 = 0$
    $f + r = 11, f \cdot r = 24$ <br> $f = 3, r = 8$ <br> $4x^2 + 8x + 3x + 6 = 0$ <br> $4x(x+2) + 3(x+2)$ <br> $(4x+3)(x+2)$ <br> $x = -2, \frac{-4}{3}$
- f. $12x^2 + 11x - 5 = 0$
    $p + d = 11, p \cdot d = -60$ <br> $p = -4, d = 15$ <br> $12x^2 -4x + 15x - 5 = 0$ <br> $4x(3x-1) + 5(3x - 1)$ <br> $(4x+5)(3x-1) = 0$ <br> $x = \frac{1}{3}, -1.25$
    
# 3.5Q

1. Solve the following quadratic equations by factorization:
- b. $2x^2 - 3x - 8 = -x^2 + 2x$
- c. $4(x^2 + 5) = 3x^2 + 10x - 4$
- d. $3x(x+5) = -(x+5)
- e.
- f.
