# 9.2J

1. Simplify each expression:
- 1. $\ln(e^3) = 3$
- 2. $\ln(e^4) = 4$
- 3. $\ln(\sqrt{e}) = \frac{1}{2}$
- 4. $\ln(\sqrt[3]{e}) = \frac{1}{3}$
- 5. $\ln(\frac{1}{e}) = -1$
- 6. $\ln(\frac{1}{e^2}) = -2$

2. Simply each expression:
- a. $e^{\ln(2)} = 2$
- b. $e^{\ln(3)} = 3$
- c. $e^{\ln(x)} = x$
- d. $e^{2 \cdot \ln(4)} = 4^2 = 16$
- e. $e^{3 \cdot \ln(x)} = x^3$
- f. $e^{-\ln(3)} = 3^{-1}$

3. Solve each of these equations:
- a. $\ln(x) = 2.7$ ; $e^{2.7} \approx 14.88$
- b. $\ln(x+1) = 1.86$ ; $x+1 = e^{1.86}$ ; $x \approx 5.42$

4. Simplify the expression $e^{x \ln(a)}$ as far as possible. <br> $a^x$

# 9.2K

2. If $p = \log_{3}(A)$ and $q = \log_{3}(B)$, find $\log_{A}(B)$ in terms of $p$ and $q$. <br> $\log_{A}(B) = \frac{q}{p}$

3. If $\log_{x}(3) = r$ and $\log_{x}(6) = s$, write each of these expressions in terms of $r$ and $s$:
- a. $\log_{3}(6) = \frac{s}{r}$
- b. $\log_{6}(3) = \frac{r}{s}$
- c. $\log_{3}(36) = \frac{2s}{r}$
- d. $\log_{3}(54) = \frac{2r + s}{r}$
- e. $\log_{9}(6) = \frac{s}{2r}$
- f. $\log_{6}(18) = \frac{s + r}{s}$
- g. $\log_{3}(2) = \frac{s - r}{r}$

4. Prove that $\log_{x}(y) = \frac{1}{\log_{y}(x)}$
  
Let $x \in \mathbb{R}\_{+}$ where $x \neq 1$. Let $y \in \mathbb{R}\_+$  $n = \log_{x}(y) $.
- Applying $\log_x$ to the equality, <br><br> $\log_y(x^n) = \log_y(y)$
<br><br>
- Because $s^1 = s$,
<br><br>
$\log_y(x^n) = 1$
<br><br>
- Through the logarithm of a power property,
<br><br>
$n \log_y(x) = 1$
<br><br>
- With $n$ isolated,
<br><br>
$n = \frac{1}{\log_y{x}}$
<br><br>
- Resubstiuting $n = \log_x(y)$ back in,
<br><br>
$\log_x(y) = \frac{1}{\log_y{x}}$
<br><br> QED or something

5. Show that $\ln(10) = \frac{1}{\log_{10}(e)}$ <br> Because $\log_{10}(10) = 1$ , $ln(10) = \frac{1}{\log_{10}(e)}$ through the change of base property. 
